A somewhat messy, cheaty proof for one case of the compatibility lemma for Apply * I am now almost entirely sure that the step-index approach works for the Apply 	case. * TODO: Make the proof and the definition of R more similar to definitions and proofs 	from the paper (Step-Indexed Syntactic Logical Relations) * TODO: Try the lambda case.

src/Language/PlutusIR/Semantics/SemanticEquivalence/Def.v
@@ -7,7 +7,8 @@ Require Import PlutusCert.Language.PlutusIR.Semantics.Dynamic.
 Require Import Arith.
 
 
-Definition terminates := fun t k => exists v j, t =[j]=> v /\ j < k.
+Definition terminates_excl := fun t j v k => t =[j]=> v /\ j < k.
+Definition terminates_incl := fun t j v k => t =[j]=> v /\ j <= k.
 
 Lemma e : forall i j k,
 i < k ->
@@ -15,6 +16,7 @@ j < k - i ->
 j < k.
 Proof. Admitted.
 
+(*
 (* Note: The cases for Ty_Forall and and Ty_IFix make use of
    type substitution and beta reduction. However, Coq can then not
    guess the decreasing argument of fix anymore. *)
@@ -50,6 +52,70 @@ Equations? R (k : nat ) (T : Ty) (t1 t2 : Term) : Prop by wf k :=
           | _ => False (* Ty_Lam, Ty_Abs and Ty_Var should not occur *)
           end.
 Proof. all: try solve [eapply e; eauto]. Qed.
+*)
+
+Equations? R (k : nat ) (T : Ty) (t1 t2 : Term) : Prop by wf k :=
+  R k T t1 t2 =>
+    emptyContext |-+ t1 : T /\
+    emptyContext |-+ t2 : T /\
+    match T with
+    | Ty_Forall X K T0 => 
+        forall v1 j1,
+          forall (Hlt_j1 : j1 < k),
+          t1 =[j1]=> v1 ->
+          exists v2 j2,
+            t2 =[j2]=> v2 /\
+            forall t0_1 t0_2 T' k',
+              forall (Hlt_k' : k' < k - j1),
+              v1 = TyAbs X K t0_1 ->
+              v2 = TyAbs X K t0_2 ->
+              emptyContext |-* T' : K ->
+              R k' (beta_reduce (substituteT X T' T0)) v1 v2
+    | Ty_Fun T1 T2 => 
+        forall v1 j1,
+          forall (Hlt_j1 : j1 < k),
+          t1 =[j1]=> v1 ->
+          exists v2 j2,
+            t2 =[j2]=> v2 /\
+            forall s1 s2 k' x1_0 x2_0 T1_0 T2_0 t1_0 t2_0 t1_0' t2_0',
+              forall (Hlt_k' : k' < k - j1),
+              v1 = LamAbs x1_0 T1_0 t1_0 ->
+              v2 = LamAbs x2_0 T2_0 t2_0 ->
+              R k' T1 s1 s2 ->
+              substitute x1_0 s1 t1_0 t1_0' ->
+              substitute x2_0 s2 t2_0 t2_0' ->
+              R k' T2 t1_0' t2_0'
+    | Ty_Builtin st => 
+        forall v1 j1,
+          forall (Hlt_j1 : j1 < k),
+          t1 =[j1]=> v1 ->
+          exists v2 j2,
+            t2 =[j2]=> v2 /\
+            v1 = v2
+    | Ty_IFix F T0 => 
+        forall v1 j1,
+          forall (Hlt_j1 : j1 < k),
+          t1 =[j1]=> v1 ->
+          exists v2 j2,
+            t2 =[j2]=> v2 /\
+            forall K k',
+              forall (Hlt_k' : k' < k - j1),
+              emptyContext |-* T0 : K ->
+              R k' (beta_reduce (unwrapIFix F K T0)) v1 v2
+    | _ => False (* Ty_Lam, Ty_Lam and Ty_Var should not occur *)
+    end.
+Proof. all: try solve [eapply e; eauto]. Qed.
+
+Definition possible_type (T : Ty) : Prop :=
+  match T with
+  | Ty_Forall _ _ _ => True
+  | Ty_Fun _ _ => True
+  | Ty_Builtin _  => True
+  | Ty_IFix _ _ => True
+  | _ => False
+  end.
+
+Definition impossible_type (T : Ty) : Prop := ~ possible_type T.
 
 Lemma R_typable_empty : forall k T t1 t2,
     R k T t1 t2 ->
@@ -66,86 +132,78 @@ Lemma R_typable_empty_2 : forall k T t1 t2,
     emptyContext |-+ t2 : T.
 Proof. intros. destruct (R_typable_empty _ _ _ _ H). assumption. Qed.
 
-Lemma R_evaluable : forall k T t1 t2,
-    terminates t1 k ->
+Lemma R_evaluable : forall k T t1 j1 v1 t2,
+    terminates_excl t1 j1 v1 k ->
+    possible_type T ->
     R k T t1 t2 ->
-    exists v1 v2 j1 j2, j1 < k /\ t1 =[j1]=> v1 /\ t2 =[j2]=> v2.
-Proof. intros. destruct H. destruct H. destruct H. autorewrite with R in H0.
-  destruct T; destruct H0 as [_ [_ [v2 [j2 [Hev2 _]]]]]; eauto; 
+    exists v2 j2, j1 < k /\ t1 =[j1]=> v1 /\ t2 =[j2]=> v2.
+Proof. intros. destruct H. autorewrite with R in H1.
+  destruct T; inversion H0; destruct H1 as [_ [_ [v2 [j2 [Hev2 _]]]]]; eauto; 
     try solve [eexists; eexists; eexists; eexists; eauto].
 Qed.
 
-Lemma R_evaluable_1 : forall k T t1 t2,
-    terminates t1 k ->
+Lemma R_evaluable_1 : forall k T t1 j1 v1 t2,
+    terminates_excl t1 j1 v1 k ->
+    possible_type T ->
     R k T t1 t2 ->
-    exists v1 j1, j1 < k /\ t1 =[j1]=> v1.
-Proof. intros. destruct (R_evaluable _ _ _ _ H H0) as [v1 [_ [j1 [_ [Hlt1 [Hev1 _]]]]]]; eauto. Qed.
+    j1 < k /\ t1 =[j1]=> v1.
+Proof. intros. destruct H. eauto. Qed.
 
-Lemma R_evaluable_2 : forall k T t1 t2,
-    terminates t1 k ->
+Lemma R_evaluable_2 : forall k T t1 j1 v1 t2,
+    terminates_excl t1 j1 v1 k ->
+    possible_type T ->
     R k T t1 t2 ->
     exists v2 j2, t2 =[j2]=> v2.
-Proof. intros. destruct (R_evaluable _ _ _ _ H H0) as [_ [v2 [_ [j2 [_ [_ Hev2]]]]]]; eauto. Qed.
+Proof. intros. destruct (R_evaluable _ _ _ _ _ _ H H0 H1) as [v2 [j2 [_ [_ Hev2]]]]; eauto. Qed.
 
-Lemma R_syntactic_equality : forall k st t1 t2,
-    terminates t1 k ->
+Lemma R_syntactic_equality : forall k st t1 j1 v1 t2,
+    terminates_excl t1 j1 v1 k ->
     R k (Ty_Builtin st) t1 t2 ->
-    exists v1 v2 j1 j2,
-      j1 < k /\
-      t1 =[j1]=> v1 /\
+    exists v2 j2,
       t2 =[j2]=> v2 /\
       v1 = v2.
-Proof. 
-  intros. destruct H. destruct H. destruct H. destruct H0 as [_ [_ [v2 [j2 [Hev2 Heq]]]]]; eauto.
-  eexists. eexists. eexists. eexists. eauto. 
-Qed.
+Proof. intros. destruct H. destruct H0 as [_ [_ [v2 [j2 [Hev2 Heq]]]]]; eauto. Qed.
 
-Lemma R_functional_extensionality : forall k T1 T2 t1 t2,
-    terminates t1 k ->
+Lemma R_functional_extensionality : forall k T1 T2 t1 j1 v1 t2,
+    terminates_excl t1 j1 v1 k ->
     R k (Ty_Fun T1 T2) t1 t2 ->
-    exists v1 v2 j1 j2,
-      j1 < k /\
-      t1 =[j1]=> v1 /\
+    exists v2 j2,
       t2 =[j2]=> v2 /\
-      (forall s1 s2 k',
+      (forall s1 s2 k' x1_0 x2_0 T1_0 T2_0 t1_0 t2_0 t1_0' t2_0',
         k' < k - j1 ->
+        v1 = LamAbs x1_0 T1_0 t1_0 ->
+        v2 = LamAbs x2_0 T2_0 t2_0 ->
         R k' T1 s1 s2 ->
-        R k' T2 (Apply v1 s1) (Apply v2 s2)).
+        substitute x1_0 s1 t1_0 t1_0' ->
+        substitute x2_0 s2 t2_0 t2_0' ->
+        R k' T2 t1_0' t2_0').
 Proof. 
-  intros k T1 T2 t1 t2 Hterm R. 
-  destruct Hterm as [v1 [j1 [Hev1 Hlt_j1]]].
+  intros k T1 T2 t1 j1 v1 t2 Hterm R. 
+  destruct Hterm.
   autorewrite with R in R.
   destruct R as [_ [_ [v2 [j2 [Hev_t2 Hfe]]]]]; eauto.
-  exists v1, v2, j1, j2. 
-  auto.
 Qed.
 
-Lemma R_unwrap : forall k F T t1 t2,
-    terminates t1 k ->
+Lemma R_unwrap : forall k F T t1 j1 v1 t2,
+    terminates_excl t1 j1 v1 k ->
     R k (Ty_IFix F T) t1 t2 ->
-    exists v1 v2 j1 j2,
-      j1 < k /\
-      t1 =[j1]=> v1 /\
+    exists v2 j2,
       t2 =[j2]=> v2 /\
       (forall K k',
         k' < k - j1 ->
         emptyContext |-* T : K ->
         R k' (beta_reduce (unwrapIFix F K T)) v1 v2).
 Proof.
-  intros k F T t1 t2 Hterm R. 
-  destruct Hterm as [v1 [j1 [Hev1 Hlt_j1]]].
+  intros k F T t1 j1 v1 t2 Hterm R.
+  destruct Hterm. 
   autorewrite with R in R.
   destruct R as [_ [_ [v2 [j2 [Hev_t2 Hunwrap]]]]]; eauto.
-  exists v1, v2, j1, j2.
-  auto.
 Qed.
 
-Lemma R_instantiational_extensionality : forall k X K T t1 t2,
-    terminates t1 k ->
+Lemma R_instantiational_extensionality : forall k X K T t1 j1 v1 t2,
+    terminates_excl t1 j1 v1 k ->
     R k (Ty_Forall X K T) t1 t2 ->
-    exists v1 v2 j1 j2,
-      j1 < k /\
-      t1 =[j1]=> v1 /\
+    exists v2 j2,
       t2 =[j2]=> v2 /\
       (forall t0_1 t0_2 T' k',
         k' < k - j1 ->
@@ -154,40 +212,23 @@ Lemma R_instantiational_extensionality : forall k X K T t1 t2,
         emptyContext |-* T' : K ->
         R k' (beta_reduce (substituteT X T' T)) v1 v2).
 Proof.
-  intros k X K T t1 t2 Hterm R. 
-  destruct Hterm as [v1 [j1 [Hev1 Hlt_j1]]].
+  intros k X K T t1 j1 v1 t2 Hterm R. 
+  destruct Hterm.
   autorewrite with R in R.
   destruct R as [_ [_ [v2 [j2 [Hev_t2 Hie]]]]]; eauto.
-  exists v1, v2, j1, j2.
-  auto.
 Qed.
 
 
 Lemma R_impossible_type : forall k t1 t2,
-    terminates t1 k ->
     (forall a, ~(R k (Ty_Var a) t1 t2)) /\
     (forall bX K T, ~(R k (Ty_Lam bX K T) t1 t2)) /\
     (forall T1 T2, ~(R k (Ty_App T1 T2) t1 t2)).
-Proof.
-  intros. destruct H. destruct H. destruct H. 
-  split; try split; try solve [intros; intro Hcon; destruct k; destruct Hcon as [_ [_ [_ [_ [_ Hfls]]]]]; eauto].
-Qed.
-
-Lemma R_impossible_k : forall t1 t2,
-    terminates t1 0 ->
-    (forall T1 T2, ~(R 0 (Ty_Fun T1 T2) t1 t2)) /\
-    (forall X K T0, ~(R 0 (Ty_Forall X K T0) t1 t2)).
-Proof.
-  intros. destruct H.
-  destruct H.
-  destruct H.
-  apply PeanoNat.Nat.nlt_0_r in H0.
-  destruct H0.
-Qed.
+Proof. intros. split; try split; try solve [intros; intro Hcon; destruct k; destruct Hcon as [_ [_ Hfls]]; eauto]. Qed.
 
 Lemma R_nontermination : forall k T t1 t2,
-    ~(terminates t1 k) ->
+    ~(exists j1 v1, terminates_excl t1 j1 v1 k) ->
+    possible_type T ->
     emptyContext |-+ t1 : T ->
     emptyContext |-+ t2 : T ->
     R k T t1 t2.
-Proof. intros. unfold terminates in H. destruct T; try solve [split; auto; split; auto; intros; exfalso; apply H; eauto]. Qed.
+Proof. intros. unfold terminates_excl in H. destruct T; try solve [split; auto; split; auto; intros; exfalso; apply H; eauto]. Qed.
